Bitmagic/WordInterval.thy
@@ -1,0 +1,285 @@
+(*  Title:      IPv4Addr.thy
+    Authors:    Julius Michaelis, Cornelius Diekmann
+*)
+theory WordInterval
+imports Main
+  NumberWang
+  "~~/src/HOL/Word/Word"
+  "~~/src/HOL/Library/Code_Target_Nat" (*!*)
+begin
+
+text{*Intervals of consecutive words*}
+
+value "(2::nat) < 2^32" (*without Code_Target_Nat, this would be really slow*)
+
+  datatype ('a::len) wordinterval = WordInterval
+                "('a::len) word" --"start (inclusive)"
+                "('a::len) word" --"end (inclusive)"
+                | RangeUnion "'a wordinterval" "'a wordinterval"
+
+  fun wordinterval_to_set :: "'a::len wordinterval \<Rightarrow> ('a::len word) set" where
+    "wordinterval_to_set (WordInterval start end) = {start .. end}" |
+    "wordinterval_to_set (RangeUnion r1 r2) = (wordinterval_to_set r1) \<union> (wordinterval_to_set r2)"
+
+  fun wordinterval_element :: "'a::len word \<Rightarrow> 'a::len wordinterval \<Rightarrow> bool" where
+    "wordinterval_element el (WordInterval s e) = (s \<le> el \<and> el \<le> e)" |
+    "wordinterval_element el (RangeUnion r1 r2) = (wordinterval_element el r1 \<or> wordinterval_element el r2)"
+  lemma wordinterval_element_set_eq[simp]: "wordinterval_element el rg = (el \<in> wordinterval_to_set rg)"
+    by(induction rg rule: wordinterval_element.induct) simp_all
+
+  fun wordinterval_union :: "'a::len wordinterval \<Rightarrow> 'a::len wordinterval \<Rightarrow> 'a::len wordinterval" where 
+    "wordinterval_union r1 r2 = RangeUnion r1 r2"
+  lemma wordinterval_union_set_eq[simp]: "wordinterval_to_set (wordinterval_union r1 r2) = wordinterval_to_set r1 \<union> wordinterval_to_set r2" by simp
+
+  fun wordinterval_empty :: "'a::len wordinterval \<Rightarrow> bool" where
+    "wordinterval_empty (WordInterval s e) = (e < s)" |
+    "wordinterval_empty (RangeUnion r1 r2) = (wordinterval_empty r1 \<and> wordinterval_empty r2)"
+  lemma wordinterval_empty_set_eq[simp]: "wordinterval_empty r \<longleftrightarrow> wordinterval_to_set r = {}"
+    by(induction r) auto
+
+  fun wordinterval_optimize_empty where
+    "wordinterval_optimize_empty (RangeUnion r1 r2) = (let r1o = wordinterval_optimize_empty r1 in (let r2o = wordinterval_optimize_empty r2 in (
+      if wordinterval_empty r1o then r2o else (if wordinterval_empty r2o then r1o else (RangeUnion r1o r2o)))))" |
+    "wordinterval_optimize_empty r = r"
+  lemma wordinterval_optimize_empty_set_eq[simp]: "wordinterval_to_set (wordinterval_optimize_empty r) = wordinterval_to_set r"
+    by(induction r) (simp_all add: Let_def)
+  lemma wordinterval_optimize_empty_double[simp]: "wordinterval_optimize_empty (wordinterval_optimize_empty r) = wordinterval_optimize_empty r"
+    apply(induction r)
+    by(simp_all add: Let_def)
+  fun wordinterval_empty_shallow where
+    "wordinterval_empty_shallow (WordInterval s e) = (e < s)" |
+    "wordinterval_empty_shallow (RangeUnion _ _) = False"
+  lemma helper_optimize_shallow: "wordinterval_empty (wordinterval_optimize_empty r) = wordinterval_empty_shallow (wordinterval_optimize_empty r)"
+    by(induction r) fastforce+
+  fun wordinterval_optimize_empty2 where
+    "wordinterval_optimize_empty2 (RangeUnion r1 r2) = (let r1o = wordinterval_optimize_empty r1 in (let r2o = wordinterval_optimize_empty r2 in (
+      if wordinterval_empty_shallow r1o then r2o else (if wordinterval_empty_shallow r2o then r1o else (RangeUnion r1o r2o)))))" |
+    "wordinterval_optimize_empty2 r = r"
+  lemma wordinterval_optimize_empty_code[code_unfold]: "wordinterval_optimize_empty = wordinterval_optimize_empty2"
+    by (subst fun_eq_iff, clarify, rename_tac r, induct_tac r)
+       (unfold wordinterval_optimize_empty.simps wordinterval_optimize_empty2.simps Let_def helper_optimize_shallow[symmetric], simp_all)
+
+  definition Empty_WordInterval :: "'a::len wordinterval" where  "Empty_WordInterval \<equiv> WordInterval 1 0"
+  lemma wordinterval_empty_Empty_WordInterval: "wordinterval_empty Empty_WordInterval" by(simp add: Empty_WordInterval_def)
+  lemma Empty_WordInterval_set_eq[simp]: "wordinterval_to_set Empty_WordInterval = {}" by(simp add: Empty_WordInterval_def)
+
+  fun wordinterval_to_list  :: "'a::len wordinterval \<Rightarrow> ('a::len wordinterval) list" where
+    "wordinterval_to_list (RangeUnion r1 r2) = wordinterval_to_list r1 @ wordinterval_to_list r2" |
+    "wordinterval_to_list r = (if wordinterval_empty r then [] else [r])"
+
+  lemma wordinterval_to_list_set_eq: "(\<Union>set (map wordinterval_to_set (wordinterval_to_list rs))) = wordinterval_to_set rs"
+  by(induction rs) simp_all
+
+  fun list_to_wordinterval where
+    "list_to_wordinterval [r] = r" |
+    "list_to_wordinterval (r#rs) = (RangeUnion r (list_to_wordinterval rs))" |
+    "list_to_wordinterval [] = Empty_WordInterval"
+
+  lemma list_to_wordinterval_set_eq: "(\<Union>set (map wordinterval_to_set rs)) = wordinterval_to_set (list_to_wordinterval rs)"
+    by(induction rs rule: list_to_wordinterval.induct) simp_all
+  
+  lemma list_to_wordinterval_set_eq_simp[simp]: "wordinterval_to_set (list_to_wordinterval (a # as)) = wordinterval_to_set (wordinterval_union a (list_to_wordinterval as))"
+    by(cases as) auto
+    
+    
+  fun wordinterval_linearize where "wordinterval_linearize rs = list_to_wordinterval (wordinterval_to_list rs)"
+  lemma "wordinterval_to_set (wordinterval_linearize r) = wordinterval_to_set r"
+    by(simp, metis list_to_wordinterval_set_eq wordinterval_to_list_set_eq)
+
+  fun wordinterval_optimize_same where "wordinterval_optimize_same rs = list_to_wordinterval (remdups (wordinterval_to_list rs))"
+  lemma wordinterval_optimize_same_set_eq[simp]: "wordinterval_to_set (wordinterval_optimize_same rs) = wordinterval_to_set rs"
+   by(simp, subst list_to_wordinterval_set_eq[symmetric]) (metis image_set wordinterval_to_list_set_eq set_remdups)
+
+  fun wordinterval_is_simple where "wordinterval_is_simple (WordInterval _ _) = True" | "wordinterval_is_simple (RangeUnion _ _) = False"
+  fun wordintervallist_union_free where
+    "wordintervallist_union_free (r#rs) = (wordinterval_is_simple r \<and> wordintervallist_union_free rs)" |
+    "wordintervallist_union_free [] = True"
+  lemma wordintervallist_union_freeX: "wordintervallist_union_free (r # rs) \<Longrightarrow> \<exists> s e. r = WordInterval s e"
+    by (induction rs) (cases r, simp, simp)+
+  lemma wordintervallist_union_free_append: "wordintervallist_union_free (a@b) = (wordintervallist_union_free a \<and> wordintervallist_union_free b)"
+    by (induction a) (auto)
+  lemma wordinterval_to_list_union_free: "l = wordinterval_to_list r \<Longrightarrow> wordintervallist_union_free l"
+    by(induction r arbitrary: l) (simp_all add: wordintervallist_union_free_append)
+
+
+
+
+  text{*previous and next words addresses, without wrap around*}
+    definition word_next :: "'a::len word \<Rightarrow> 'a::len word" where
+      "word_next a \<equiv> if a = max_word then max_word else a + 1"
+    definition word_prev :: "'a::len word \<Rightarrow> 'a::len word" where
+      "word_prev a \<equiv> if a = 0 then 0 else a - 1"
+  
+    lemma "word_next (2:: 8 word) = 3" by eval
+    lemma "word_prev (2:: 8 word) = 1" by eval
+    lemma "word_prev (0:: 8 word) = 0" by eval
+
+
+  fun wordinterval_setminus :: "'a::len wordinterval \<Rightarrow> 'a::len wordinterval \<Rightarrow> 'a::len wordinterval" where
+    "wordinterval_setminus (WordInterval s e) (WordInterval ms me) = (
+      if s > e \<or> ms > me then WordInterval s e else
+      if me \<ge> e
+        then
+          WordInterval (if ms = 0 then 1 else s) (min e (word_prev ms))
+        else if ms \<le> s
+        then
+          WordInterval (max s (word_next me)) (if me = max_word then 0 else e)
+        else
+          RangeUnion (WordInterval (if ms = 0 then 1 else s) (word_prev ms)) (WordInterval (word_next me) (if me = max_word then 0 else e))
+        )" |
+     "wordinterval_setminus (RangeUnion r1 r2) t = RangeUnion (wordinterval_setminus r1 t) (wordinterval_setminus r2 t)"|
+     "wordinterval_setminus t (RangeUnion r1 r2) = wordinterval_setminus (wordinterval_setminus t r1) r2"
+
+  lemma wordinterval_setminus_rr_set_eq[simp]: "wordinterval_to_set(wordinterval_setminus (WordInterval s e) (WordInterval ms me)) = 
+    wordinterval_to_set (WordInterval s e) - wordinterval_to_set (WordInterval ms me)"
+     apply(simp only: wordinterval_setminus.simps)
+     apply(case_tac "e < s") 
+      apply simp
+     apply(case_tac "me < ms") 
+      apply simp
+     apply(case_tac [!] "e \<le> me")
+      apply(case_tac [!] "ms = 0") 
+        apply(case_tac [!] "ms \<le> s") 
+            apply(case_tac [!] "me = max_word")
+                    apply(simp_all add: word_prev_def word_next_def min_def max_def)
+            apply(safe)
+                                  apply(auto)
+                          apply(uint_arith) 
+                         apply(uint_arith)
+                        apply(uint_arith)
+                       apply(uint_arith)
+                      apply(uint_arith)
+                     apply(uint_arith)
+                    apply(uint_arith)
+                   apply(uint_arith)
+                  apply(uint_arith)
+                 apply(uint_arith)
+                apply(uint_arith)
+               apply(uint_arith)
+              apply(uint_arith)
+             apply(uint_arith)
+            apply(uint_arith)
+           apply(uint_arith)
+          apply(uint_arith)
+         apply(uint_arith)
+        apply(uint_arith)
+       apply(uint_arith)
+      apply(uint_arith)
+     apply(uint_arith)
+   done
+
+  lemma wordinterval_setminus_set_eq[simp]: "wordinterval_to_set (wordinterval_setminus r1 r2) = 
+    wordinterval_to_set r1 - wordinterval_to_set r2"
+    apply(induction rule: wordinterval_setminus.induct)
+      using wordinterval_setminus_rr_set_eq apply blast
+     apply auto
+    done
+  lemma wordinterval_setminus_empty_struct: "wordinterval_empty r2 \<Longrightarrow> wordinterval_setminus r1 r2 = r1"
+    by(induction r1 r2 rule: wordinterval_setminus.induct) auto
+
+  definition "wordinterval_UNIV \<equiv> WordInterval 0 max_word"
+  lemma wordinterval_UNIV_set_eq[simp]: "wordinterval_to_set wordinterval_UNIV = UNIV"
+    unfolding wordinterval_UNIV_def
+    using max_word_max by fastforce
+    
+  fun wordinterval_invert :: "'a::len wordinterval \<Rightarrow> 'a::len wordinterval" where
+    "wordinterval_invert r = wordinterval_setminus wordinterval_UNIV r"
+  lemma wordinterval_invert_set_eq[simp]: "wordinterval_to_set (wordinterval_invert r) = UNIV - wordinterval_to_set r" by(auto)
+
+  lemma wordinterval_invert_UNIV_empty: "wordinterval_empty (wordinterval_invert wordinterval_UNIV)" by simp
+
+  fun wordinterval_intersection :: "'a::len wordinterval \<Rightarrow> 'a::len wordinterval \<Rightarrow> 'a::len wordinterval" where 
+    "wordinterval_intersection r1 r2 = 
+      wordinterval_optimize_same (wordinterval_setminus (wordinterval_union r1 r2) (wordinterval_union (wordinterval_invert r1) (wordinterval_invert r2)))"
+  lemma wordinterval_intersection_set_eq[simp]: "wordinterval_to_set (wordinterval_intersection r1 r2) = wordinterval_to_set r1 \<inter> wordinterval_to_set r2"
+    unfolding wordinterval_intersection.simps wordinterval_optimize_same_set_eq by auto
+  
+  lemma wordinterval_setminus_intersection_empty_struct_rr: 
+    "wordinterval_empty (wordinterval_intersection (WordInterval r1s r1e) (WordInterval r2s r2e)) \<Longrightarrow> 
+    wordinterval_setminus (WordInterval r1s r1e) (WordInterval r2s r2e) = (WordInterval r1s r1e)"
+    apply(subst(asm) wordinterval_empty_set_eq) 
+    apply(subst(asm) wordinterval_intersection_set_eq)
+    apply(unfold wordinterval_to_set.simps(1))
+    apply(cases "wordinterval_empty (WordInterval r1s r1e)", case_tac [!] "wordinterval_empty (WordInterval r2s r2e)")
+       apply(unfold wordinterval_empty.simps(1))
+       apply(force, force, force)
+    apply(cases "r1e < r2s") 
+     defer
+     apply(subgoal_tac "r2e < r1s")
+      defer
+      apply force
+     apply(simp only: wordinterval_setminus.simps)
+     apply(case_tac [!] "r1e \<le> r2e", case_tac [!] "r2s \<le> r1s")
+           apply(auto)
+     apply(metis (hide_lams, no_types) comm_semiring_1_class.normalizing_semiring_rules(24) inc_i word_prev_def le_minus min.absorb_iff1 word_le_sub1 word_zero_le)
+    apply(metis inc_le word_next_def max.order_iff)
+  done
+
+  declare wordinterval_intersection.simps[simp del]
+  declare wordinterval_setminus.simps(1)[simp del]
+
+  lemma wordinterval_setminus_intersection_empty_struct:
+    "wordinterval_empty (wordinterval_intersection r1 r2) \<Longrightarrow> 
+    wordinterval_setminus r1 r2 = r1"
+    by (induction r1 r2 rule: wordinterval_setminus.induct, auto simp add: wordinterval_setminus_intersection_empty_struct_rr) fastforce
+
+  definition wordinterval_subset :: "'a::len wordinterval \<Rightarrow> 'a::len wordinterval \<Rightarrow> bool" where
+    "wordinterval_subset r1 r2 \<equiv> wordinterval_empty (wordinterval_setminus r1 r2)"
+  lemma wordinterval_subset_set_eq[simp]: "wordinterval_subset r1 r2 = (wordinterval_to_set r1 \<subseteq> wordinterval_to_set r2)"
+    unfolding wordinterval_subset_def by simp
+
+  definition wordinterval_eq :: "'a::len wordinterval \<Rightarrow> 'a::len wordinterval \<Rightarrow> bool" where 
+    "wordinterval_eq r1 r2 = (wordinterval_subset r1 r2 \<and> wordinterval_subset r2 r1)"
+  lemma wordinterval_eq_set_eq: "wordinterval_eq r1 r2 \<longleftrightarrow> wordinterval_to_set r1 = wordinterval_to_set r2"
+    unfolding wordinterval_eq_def by auto
+  thm iffD1[OF wordinterval_eq_set_eq]
+  declare iffD1[OF wordinterval_eq_set_eq, simp]
+  lemma wordinterval_eq_comm: "wordinterval_eq r1 r2 \<longleftrightarrow> wordinterval_eq r2 r1"
+    unfolding wordinterval_eq_def by fast
+  lemma wordinterval_to_set_alt: "wordinterval_to_set r = {x. wordinterval_element x r}"
+    unfolding wordinterval_element_set_eq by blast
+ 
+  lemma wordinterval_un_empty: "wordinterval_empty r1 \<Longrightarrow> wordinterval_eq (wordinterval_union r1 r2) r2"
+    by(subst wordinterval_eq_set_eq, simp)
+  lemma wordinterval_un_emty_b: "wordinterval_empty r2 \<Longrightarrow> wordinterval_eq (wordinterval_union r1 r2) r1"
+    by(subst wordinterval_eq_set_eq, simp)
+  
+  lemma wordinterval_Diff_triv: 
+    assumes "wordinterval_empty (wordinterval_intersection a b)" shows "wordinterval_eq (wordinterval_setminus a b) a"
+    using wordinterval_setminus_intersection_empty_struct[OF assms] wordinterval_eq_set_eq[of a a] by simp
+
+  fun wordinterval_size where
+    "wordinterval_size (RangeUnion a b) = wordinterval_size a + wordinterval_size b" |
+    "wordinterval_size (WordInterval s e) = (if s \<le> e then 1 else 0)"
+  lemma "wordinterval_size r = length (wordinterval_to_list r)"
+    by(induction r, simp_all)
+
+  lemma [simp]: "\<exists>x::('a::len wordinterval). y \<in> wordinterval_to_set x"
+  proof show "y \<in> wordinterval_to_set wordinterval_UNIV" by simp qed
+
+
+
+
+
+  lemma wordinterval_eq_reflp:
+    "reflp wordinterval_eq"
+    apply(rule reflpI)
+    by(simp only: wordinterval_eq_set_eq)
+  lemma wordintervalt_eq_symp:
+    "symp wordinterval_eq"
+    apply(rule sympI)
+    by(simp add: wordinterval_eq_comm)
+  lemma wordinterval_eq_transp:
+    "transp wordinterval_eq"
+    apply(rule transpI)
+    by(simp only: wordinterval_eq_set_eq)
+
+  lemma wordinterval_eq_equivp:
+    "equivp wordinterval_eq"
+    by (auto intro: equivpI wordinterval_eq_reflp wordintervalt_eq_symp wordinterval_eq_transp)
+(*
+  quotient_type 'a bitrrq = "'a::len wordinterval" / "wordinterval_eq"
+    by (rule wordinterval_eq_equivp)
+*)
+    
+end
