Examples/Example_Semantics.thy
@@ -58,8 +58,8 @@ text{*we use a primitive matcher which always apllies.*}
 
   text{*We tune the primitive matcher to support everything we need in the example. Note that the undefined cases cannot be handled with these exact semantics!*}
   fun applies_exampleMatchExact :: "(iptrule_match, packet) matcher" where
-  "applies_exampleMatchExact (Src (Ip4Addr addr)) p \<longleftrightarrow> src_ip p = (ipv4addr_of_dotteddecimal addr)" |
-  "applies_exampleMatchExact (Dst (Ip4Addr addr)) p \<longleftrightarrow> dst_ip p = (ipv4addr_of_dotteddecimal addr)" |
+  "applies_exampleMatchExact (Src (Ip4Addr addr)) p \<longleftrightarrow> src_ip p = (ipv4addr_of_dotdecimal addr)" |
+  "applies_exampleMatchExact (Dst (Ip4Addr addr)) p \<longleftrightarrow> dst_ip p = (ipv4addr_of_dotdecimal addr)" |
   "applies_exampleMatchExact (Prot ProtAll) p \<longleftrightarrow> True" |
   "applies_exampleMatchExact (Prot ipt_protocol.ProtTCP) p \<longleftrightarrow> prot p = protPacket.ProtTCP" |
   "applies_exampleMatchExact (Prot ipt_protocol.ProtUDP) p \<longleftrightarrow> prot p = protPacket.ProtUDP"
@@ -69,14 +69,14 @@ text{*we use a primitive matcher which always apllies.*}
                           Rule (Match (Dst (Ip4Addr (0,0,0,0)))) Log, 
                           Rule (Match (Prot ipt_protocol.ProtTCP)) Accept,
                           Rule (Match (Prot ipt_protocol.ProtTCP)) Drop]
-         ],applies_exampleMatchExact,\<lparr>src_ip=(ipv4addr_of_dotteddecimal (1,2,3,4)), dst_ip=(ipv4addr_of_dotteddecimal (0,0,0,0)), prot=protPacket.ProtTCP\<rparr>\<turnstile>
+         ],applies_exampleMatchExact,\<lparr>src_ip=(ipv4addr_of_dotdecimal (1,2,3,4)), dst_ip=(ipv4addr_of_dotdecimal (0,0,0,0)), prot=protPacket.ProtTCP\<rparr>\<turnstile>
             \<langle>[Rule MatchAny (Call ''FORWARD'')], Undecided\<rangle> \<Rightarrow> (Decision FinalAllow)"
   apply(rule call_result)
   apply(auto)
   apply(rule Semantics.seq_cons)
-  apply(auto intro: Semantics.nomatch simp add: ipv4addr_of_dotteddecimal.simps ipv4addr_of_nat_def)
+  apply(auto intro: Semantics.nomatch simp add: ipv4addr_of_dotdecimal.simps ipv4addr_of_nat_def)
   apply(rule Semantics.seq_cons)
-  apply(auto intro: Semantics.log simp add: ipv4addr_of_dotteddecimal.simps ipv4addr_of_nat_def)
+  apply(auto intro: Semantics.log simp add: ipv4addr_of_dotdecimal.simps ipv4addr_of_nat_def)
   apply(rule Semantics.seq_cons)
   apply(auto intro: Semantics.accept)
   apply(auto intro: Semantics.decision)
