Examples/Ringofsaturn_com/Analyze_Ringofsaturn_com.thy
@@ -26,7 +26,7 @@ text{* We have directly executable approximating semantics: @{thm approximating_
   value "simple_ruleset example_ruleset_simplified"
 
 
-  lemma "approximating_bigstep_fun (simple_matcher, in_doubt_allow) \<lparr>src_ip=ipv4addr_of_dotteddecimal (192,168,3,5), dst_ip=0, prot=protPacket.ProtTCP\<rparr>
+  lemma "approximating_bigstep_fun (simple_matcher, in_doubt_allow) \<lparr>src_ip=ipv4addr_of_dotdecimal (192,168,3,5), dst_ip=0, prot=protPacket.ProtTCP\<rparr>
         example_ruleset_simplified
         Undecided = Decision FinalAllow" by eval
   hide_const example_ruleset_simplified example_ruleset
@@ -123,7 +123,7 @@ done
 value(code) "approximating_bigstep_fun (simple_matcher, in_doubt_allow) \<lparr>src_ip=0, dst_ip=0, prot=protPacket.ProtTCP\<rparr>
           simple_example_firewall
          Undecided"
-value(code) "approximating_bigstep_fun (simple_matcher, in_doubt_allow) \<lparr>src_ip=ipv4addr_of_dotteddecimal (192,168,3,5), dst_ip=0, prot=protPacket.ProtTCP\<rparr>
+value(code) "approximating_bigstep_fun (simple_matcher, in_doubt_allow) \<lparr>src_ip=ipv4addr_of_dotdecimal (192,168,3,5), dst_ip=0, prot=protPacket.ProtTCP\<rparr>
         simple_example_firewall
         Undecided"
 
